%%%%%%%%%%%%%%%%%%%%%%
% Preamble %%%%%%%%%%%
\input{preamble.tex}

%%%%%%%%%%%%%%%%%%%%%%
% Main Document %%%%%%
\begin{document}

%%%%%%%%%%%%%%%%%%%%%%
% Document header %%%%
{\LARGE \centering ECON 21020 -- Problem Set 3\par}
{\vspace{-1em} \large \centering Alex Ding \par}
{\centering \vspace{-1em} \today \par }

%%%%%%%%%%%%%%%%%%%%%%
% Problem 1 %%%%%%%%%%

\section{}

\textbf{1.1}

False,

\section{}

\textbf{2.5}

ATT would make more sense than ATE because the offenders are about to be sent to confinement.

\textbf{2.6}

ATE = ATT P(W=1) + ATU P(W=0)

-0.2 = 0.6 * ATT + 0.4 * ATU

-0.2 - 0.6 * ATT = 0.4 * ATU

- 1 - 3 * ATT = 2 * ATU

-3 ATT = 2 * ATU + 1

ATT = -2/3 ATU - 1/3

Substitute (-1,1) for ATU

Range of ATT: (1/3,-1)

\textbf{2.7}

ATT $\leq$ ATU

ATU $\geq$ -2/3 ATU - 1/3

5/3 ATU $\geq$ - 1/3

ATU $\geq$ - 1/5

Substitute (-1/5, 1) for ATU

Range of ATT: (-1/5, -1)

\newpage
\section{}

\textbf{5.2}

E[X $\mid$ X $\geq$ t] = $\int_{t}^{1}$ x *(1/(1-t)) dx 

= $x^{2}/(2(1-t)$ from t to 1: 

= 1-2(1-t) - $(t^{2}/2(1-t) = 1/2(t+1)

E[X $\mid$ X $<$ t] = $\int_{-1}^{t}$ x(1/t-(-1)) dx = $x^{2}/2(t+1)$ from -1 to t:

= $t^{2}$/2(t+1) - (1/2(t+1)) = $t^{2} - 1$/2(t+1) = 1/2(t-1)

P[X $\geq$ t] = 1/2(1-t)

P[X $\leq$ t] = 1/2(1+t)

Var(X) = 1/12(2)^2 = 1/3
 
\textbf{5.3}

By Yitzhaki's Theorem:

w(t) = (E[X $\mid$ X $\geq$ t] - E[X $\mid$ X $<$ t]) * P[X $\geq$ t] * P[X $\leq$ t] / Var(X)

w(t) = $((t+1)/2 - (t-1)/2) * (1/2-1/2t) * (1/2+1/2t) = 3/2(1-t^{2}) 

\textbf{5.4}

By Yitzhaki's Theorem:

$\beta$ = $\int_{-\infty}^{\infty}$ (d/dt E[Y $\mid$ X = t]) w(t) dt

$\beta$ = $\int_{-1}^{1}$ $t^{3}$ (3/2) * $(1 - t^{2})$ dt

$\beta$ = 3/2 $\int_{-1}^{1}$ $3t^{2}$ * $1 - t^{2}$ dt

$\beta$ = 3/2 $t^{3}$ - (3/5)$t^{5}$ = 3/2 * (1 - 3/5) - (-1 + 3/5) = 3/2 * 4/5 = 6/5

\textbf{5.5}

E[d/dx E[Y $\mid$ X]] = $\int_{0}^{1}$ d/dx E[Y $\mid$ X = t]dt =  $\int_{0}^{1}$ 3/2 * $t^2$ dt = $t^{3}$ from 0 to 1 = 1 - 0 = 1.

1 $\neq$ 6/5, so therefore $\beta$ does not equal to the average derivative of the condition expectation function.

\section{}
\textbf{1.1}
E[$\epsilon \mid X]$ = E[Y-E[Y$\mid$X]$\mid$ X] = E[Y$\mid$X]] - E[E[Y$\mid$X]$\mid$ X] = 0 by law of iterated expectations.
\end{document}